PAC: add quicksort impl

PAC/PAC_Checker_Synthesis.thy
@@ -77,7 +77,7 @@ lemma term_order_rel[def_pat_rules]:
 
 lemma term_order_rel_alt_def:
   \<open>term_order_rel = lexord (p2rel char.lexordp)\<close>
-  by (auto simp: p2rel_def char.lexordp_conv_lexord intro!: arg_cong[of _ _ lexord])
+  by (auto simp: p2rel_def char.lexordp_conv_lexord var_order_rel_def intro!: arg_cong[of _ _ lexord])
 
 
 instantiation char :: linorder
@@ -121,7 +121,7 @@ proof -
     \<open>term_order_rel' x y \<longleftrightarrow> x < y\<close>
     unfolding less_than_char_of_char[symmetric, abs_def]
     by (auto simp: lexordp_conv_lexord less_eq_list_def
-         less_list_def lexordp_def
+         less_list_def lexordp_def var_order_rel_def
          rel2p_def term_order_rel_alt_def p2rel_def)
 qed
 
@@ -230,13 +230,47 @@ sepref_definition add_poly_impl
   by sepref
 
 
+
+definition full_quicksort_poly where
+  \<open>full_quicksort_poly = full_quicksort_ref (\<lambda>x y. x = y \<or> (x, y) \<in> term_order_rel) fst\<close>
+
+lemma down_eq_id_list_rel: \<open>\<Down>(\<langle>Id\<rangle>list_rel) x = x\<close>
+  by auto
+
+definition quicksort_poly:: \<open>nat \<Rightarrow> nat \<Rightarrow> llist_polynom \<Rightarrow> (llist_polynom) nres\<close> where
+  \<open>quicksort_poly x y  z = quicksort_ref (\<le>) fst (x, y, z)\<close>
+
+term partition_between_ref
+
+definition partition_between_poly :: \<open>nat \<Rightarrow> nat \<Rightarrow> llist_polynom \<Rightarrow> (llist_polynom \<times> nat) nres\<close> where
+  \<open>partition_between_poly = partition_between_ref (\<le>) fst\<close>
+
+definition partition_main_poly :: \<open>nat \<Rightarrow> nat \<Rightarrow> llist_polynom \<Rightarrow> (llist_polynom \<times> nat) nres\<close> where
+  \<open>partition_main_poly = partition_main (\<le>)  fst\<close>
+
 lemma full_quicksort_sort_poly_spec:
-  \<open>full_quicksort (\<lambda>x y. x = y \<or> (x, y) \<in> lexord var_order_rel) fst xs
+  \<open>full_quicksort_poly xs
     \<le> sort_poly_spec xs\<close>
 proof -
+  have xs: \<open>(xs, xs) \<in> \<langle>Id\<rangle>list_rel\<close> and \<open>\<Down>(\<langle>Id\<rangle>list_rel) x = x\<close> for x
+    by auto
   show ?thesis
+    unfolding full_quicksort_poly_def
+    apply (rule full_quicksort_ref_full_quicksort[THEN fref_to_Down_curry, THEN order_trans])
+    subgoal
+      apply (auto simp: rel2p_def var_order_rel_def p2rel_def Relation.total_on_def)
+      apply (smt PAC_Checker_Synthesis.less_char_def char.less_trans less_than_char_def lexord_partial_trans p2rel_def)
+      done
+    subgoal
+      using total_on_lexord_less_than_char_linear[unfolded var_order_rel_def]
+      apply (auto simp: rel2p_def var_order_rel_def p2rel_def Relation.total_on_def
+        PAC_Checker_Synthesis.less_char_def)
+      done
+    subgoal by fast
+    apply (rule xs)
+    apply (subst down_eq_id_list_rel)
     unfolding sorted_wrt_map sort_poly_spec_def
-    apply (rule full_quicksort_correct_sorted[where R = \<open>(\<lambda>x y. x = y \<or> (x, y) \<in> lexord var_order_rel)\<close> and h = \<open>fst\<close>,
+    apply (rule full_quicksort_correct_sorted[where R = \<open>(\<lambda>x y. x = y \<or> (x, y) \<in> term_order_rel)\<close> and h = \<open>fst\<close>,
        THEN order_trans])
     subgoal
       apply (auto simp: rel2p_def var_order_rel_def p2rel_def Relation.total_on_def)
@@ -251,5 +285,61 @@ proof -
     by (auto simp: rel2p_def p2rel_def)
    done
 qed
+
+lemma le_term_order_rel':
+  \<open>(\<le>) = (\<lambda>x y. x = y \<or>  term_order_rel' x y)\<close>
+  apply (intro ext)
+  apply (auto simp add: less_list_def less_eq_list_def
+    lexordp_eq_conv_lexord lexordp_def)
+  using term_order_rel'_alt_def_lexord term_order_rel'_def apply blast
+  using term_order_rel'_alt_def_lexord term_order_rel'_def apply blast
+  done
+
+sepref_definition partition_main_poly_impl
+  is \<open>uncurry2 partition_main_poly\<close>
+  :: \<open>nat_assn\<^sup>k *\<^sub>a nat_assn\<^sup>k *\<^sub>a poly_assn\<^sup>k \<rightarrow>\<^sub>a prod_assn poly_assn nat_assn \<close>
+  unfolding partition_main_poly_def partition_main_def
+    term_order_rel'_def[symmetric]
+    term_order_rel'_alt_def
+    le_term_order_rel'
+  by sepref
+
+declare partition_main_poly_impl.refine[sepref_fr_rules]
+
+sepref_definition partition_between_poly_impl
+  is \<open>uncurry2 partition_between_poly\<close>
+  :: \<open>nat_assn\<^sup>k *\<^sub>a nat_assn\<^sup>k *\<^sub>a poly_assn\<^sup>k \<rightarrow>\<^sub>a prod_assn poly_assn nat_assn \<close>
+  unfolding partition_between_poly_def partition_between_ref_def
+    partition_main_poly_def[symmetric]
+  unfolding choose_pivot3_def
+    term_order_rel'_def[symmetric]
+    term_order_rel'_alt_def choose_pivot_def
+    le_term_order_rel'
+  by sepref
+
+declare partition_between_poly_impl.refine[sepref_fr_rules]
+
+
+sepref_definition quicksort_poly_impl
+  is \<open>uncurry2 quicksort_poly\<close>
+  :: \<open>nat_assn\<^sup>k *\<^sub>a nat_assn\<^sup>k *\<^sub>a poly_assn\<^sup>k \<rightarrow>\<^sub>a poly_assn\<close>
+  unfolding partition_main_poly_def quicksort_ref_def quicksort_poly_def
+    partition_between_poly_def[symmetric]
+  by sepref
+
+declare quicksort_poly_impl.refine[sepref_fr_rules]
+
+sepref_register quicksort_poly
+sepref_definition full_quicksort_poly_impl
+  is \<open>full_quicksort_poly\<close>
+  :: \<open>poly_assn\<^sup>k \<rightarrow>\<^sub>a poly_assn\<close>
+  unfolding full_quicksort_poly_def full_quicksort_ref_def
+    quicksort_poly_def[symmetric]
+    le_term_order_rel'[symmetric]
+    term_order_rel'_def[symmetric]
+    List.null_def
+  by sepref
+
+
 
 end
