PAC/PAC_Checker.thy
@@ -375,6 +375,10 @@ lemma less_than_char_of_char[code_unfold]:
   \<open>(x, y) \<in> less_than_char \<longleftrightarrow> (of_char x :: nat) < of_char y\<close>
   by (auto simp: less_than_char_def less_char_def)
 
+
+lemmas [code] = 
+  add_poly_l'.simps[unfolded var_order_rel_def]
+
 export_code add_poly_l' in SML module_name test
 
 
